---
tags:
  - cs1200LN
date: {}
---
#cs1200LN
|  |  |  |  |
|----------|----------|----------|----------|
| [[CS1200|Home]] | [[CS1200 Calendar|Calendar]] | [[CS1200 Syllabus]] | [[Lecture Notes]] |


## Reminders

```query
cs1200task
where done = false
order by pos
limit 4
render [[template/topic]]
```

## Objectives

```query
task
where page = "CS1200 Calendar" and done = false
limit 3
order by pos
render [[template/topic]]
```
---


# Summations and Products of Sequences

In addition to calculating individual terms of a sequence, it is often helpful to denote the sum or product of consecutive terms.

## Summation Notation vs Expanded Form

#Definition if m and n are integers and m <= n, then the symbol
```latex
\sum_{k=m}^na_k
```
read as the **summation form from k equals m to n of a-sub-k**, is the sum of all terms in the sequence.
```latex
a_m + a_{m+1} + a_{m+2} + ... + a_n
```
is known as the **expanded form** of the sum and is equivalent to the summation form
```latex
\sum_{k=m}^na_k = a_m + a_{m+1} + a_{m+2} + ... + a_n
```

In the example above, **k** is the **index** of the summation, 
**m** is the **lower limit** of the summation, 
and **n** is the **upper limit** of the summation


## Changing End Terms of a Summation

Often times, summations require adjustment to better suit a mathematical argument or to adhere to some known theorem. Weâ€™ll go over some common methods of working with summations here

_examples:_

**Re-write as a summation from 1 to n**
```latex
\sum_{i=1}^{n+1}\frac{1}{i^2}
```

_ans:_

```latex
\frac{1}{(n+1)^2} + \sum_{i=1}^n\frac{1}{i^2}
```

**Express as a single summation**
```latex
\sum_{k=0}^n2^k + 2^{n+1}
```

_ans:_

```latex
\sum_{k=0}^{n+1}2^k
```


## Changing the Variables of a Sequence

In addition to adding and removing terms from the summation notation, you can also perform a change of variables on the _index_ of the sum.

_example:_

**Change to index j where j = k+1**
```latex
\sum_{k=0}^6\frac{1}{k+1}
```

_ans:_

```latex
\sum_{j=1}^7\frac{1}{j}
```

Donâ€™t forget to change all three of:
* The expression for the k-th / j-th term
* The lower limit
* The upper limit

#DiscussionQuestion How can we express the following as a sum with a lower limit of 1?
```latex
\sum_{k=0}^n \frac{k+1}{n+k}
```

* [ ] joseph  ðŸ“…2024-06-18 #cs1200EC


let j = k+1
```latex
\sum_{j=1}^{n+1} \frac{j}{n+j-1}
```


## Telescoping sums

_notice the following:_
```latex
\frac{1}{k}-\frac{1}{k+1} = \frac{k+1}{k(k+1)}-\frac{k}{k(k+1)} = \frac{1}{k(k+1)}
```

This gives a unique property to summations of the form
```latex
\sum_{k=1}^n\frac{1}{k(k+1)} = \sum_{k=1}^n(\frac{1}{k}-\frac{1}{k+1})
```

Expanding this sum we see that certain terms cancel each other
```latex
(\frac{1}{1} - \frac{1}{2}) + (\frac{1}{2} - \frac{1}{3}) + ... + (\frac{1}{n} - \frac{1}{n+1})
```
By associativity of the real numbers is equal to...
```latex
\frac{1}{1} + (- \frac{1}{2} + \frac{1}{2}) + (- \frac{1}{3} + \frac{1}{3}) + ... + (- \frac{1}{n} + \frac{1}{n}) - \frac{1}{n+1}
```

Which leaves us with a formula of
```latex
\sum_{k=1}^n\frac{1}{k(k+1)} = 1 - \frac{1}{n+1}
```

#Definition A sum is said to have a **closed form** expression if it can be shown to be equal to a formula not containing ellipsis(**...**) or summation symbols(**âˆ‘**)

## Product notation

#Definition If m and n are integers and m <= n, then the symbol
```latex
\prod_{k=m}^na_k
```
read as the **product from k equals m to n of a-sub-k**, is the product of all terms in the sequence
```latex
\prod_{k=m}^na_k = a_m*a_{m+1}*a_{m+2}* ... *a_n
```

_example:_
```latex
\prod_{k=1}^5a_k = a_1a_2a_3a_4a_5
```

#Definition For each positive integer n, the quantity **n factorial**, denoted **n!**, is defined as the product of all the integers from 1 to n.
```latex
n! = \prod_{k=1}^nk = n*(n-1)* ... *3*2*1
```
The **zero factorial**, denoted **0!**, is defined to be 1
```latex
0! = 1
```

## Properties of sums and products

#Theorem Given any two sequences of real numbers
```latex
a_m, a_{m+1}, a_{m+2}, ... \quad\text{ and }\quad b_m, b_{m+1}, b_{m+2}, ...
```
The following statements hold for any integer n >= m
```latex
\sum^n_{k=m}a_k + \sum_{k=m}^nb_k = \sum_{k=m}^n(a_k + b_k)
```
```latex
c\times\sum_{k=m}^na_k = \sum_{k=m}^nc\times a_k
```
Where c is any real number
```latex
(\prod_{k=m}^na_k)*(\prod_{k=m}^nb_k) = \prod_{k=m}^n(a_k*b_k)
```

#BoardQuestion Let a_k = k+1 and b_k = k-1 for all integers k

Write the following as a single summation
```latex
\sum_{k=m}^na_k + 2*\sum_{k=m}^nb_k
```

_theorem 2_
```latex
\sum_{k=m}^na_k + \sum_{k=m}^n2*b_k
```

_theorem 1_
```latex
\sum_{k=m}^{n} (a_k + 2*b_k) 
```

_theorem 2_
```latex
2\times\sum_{k=m}^{n} (0.5*a_k + b_k) 
```

* [ ] brileigh, joseph  ðŸ“…2024-06-18 #cs1200EC
